cedar-lean/Cedar/Thm/Frontend/CstSlice.lean
@@ -56,7 +56,7 @@ private theorem varBoundWF_of_toPRScope? {v : Cst.VariableDef} (h : (v.toPRScope
         cases hu : e.toEntityUID? with
         | none => rw [hu] at h; simp at h
         | some x => simp [varBoundWF, hineq, het, hu]
-      | rLess | rLessEq | rGreater | rGreaterEq | rNotEq =>
+      | rLess | rLessEq | rGreater | rGreaterEq | rNotEq | rInvalidSingleEq =>
         simp [Cst.VariableDef.toPRScope?, hineq, het] at h
     | some t =>
       cases op with
@@ -65,7 +65,7 @@ private theorem varBoundWF_of_toPRScope? {v : Cst.VariableDef} (h : (v.toPRScope
         cases hu : e.toEntityUID? with
         | none => rw [hu] at h; simp at h
         | some x => simp [varBoundWF, hineq, het, hu]
-      | rEq | rLess | rLessEq | rGreater | rGreaterEq | rNotEq =>
+      | rEq | rLess | rLessEq | rGreater | rGreaterEq | rNotEq | rInvalidSingleEq =>
         simp [Cst.VariableDef.toPRScope?, hineq, het] at h
 
 private theorem toPrincipalScope?_inv {v : Cst.VariableDef} {ps : PrincipalScope}
@@ -170,7 +170,7 @@ private theorem varBound?_eq_scope_bound {v : Cst.VariableDef} {scope : Scope}
           Option.some.injEq] at h
         obtain ⟨eref, hu, hsc⟩ := h; subst hsc
         simp [varBound?, hineq, het, Scope.bound, hu]
-      | rLess | rLessEq | rGreater | rGreaterEq | rNotEq =>
+      | rLess | rLessEq | rGreater | rGreaterEq | rNotEq | rInvalidSingleEq =>
         simp [Cst.VariableDef.toPRScope?, hineq, het] at h
     | some t =>
       cases op with
@@ -179,7 +179,7 @@ private theorem varBound?_eq_scope_bound {v : Cst.VariableDef} {scope : Scope}
           Option.some.injEq] at h
         obtain ⟨eref, hu, ety, _, hsc⟩ := h; subst hsc
         simp [varBound?, hineq, het, Scope.bound, hu]
-      | rEq | rLess | rLessEq | rGreater | rGreaterEq | rNotEq =>
+      | rEq | rLess | rLessEq | rGreater | rGreaterEq | rNotEq | rInvalidSingleEq =>
         simp [Cst.VariableDef.toPRScope?, hineq, het] at h
 
 private theorem toPrincipalScope?_some {v : Cst.VariableDef} {ps : PrincipalScope}
@@ -312,7 +312,7 @@ private theorem scope_slice_translate
             if satisfiedBound (Cst.scopeAnalysis x.1 (hwf x.1 x.2)) req entities
             then some x.1 else none) hF,
           List.filterMap_map, List.filter_cons]
-        simp only [hb, Bool.false_eq_true, if_false]
+        simp only [hb, Bool.false_eq_true, ite_false]
         exact ihtl
       · have hF : (fun x : {x // x ∈ hd :: tl} =>
             if satisfiedBound (Cst.scopeAnalysis x.1 (hwf x.1 x.2)) req entities
@@ -323,7 +323,7 @@ private theorem scope_slice_translate
             if satisfiedBound (Cst.scopeAnalysis x.1 (hwf x.1 x.2)) req entities
             then some x.1 else none) hF,
           List.filterMap_map, List.filter_cons]
-        simp only [hb, if_true]
+        simp only [hb, ite_true]
         exact mapM_toPolicy?_cons hhd ihtl
 
 /-- The CST scope-based slice and the AST scope-based slice choose the same
