cedar-lean/Cedar/Thm/Frontend/Translation/PolicyToExpr.lean
@@ -575,6 +575,7 @@ theorem action_leaf_eq {va : Cst.VariableDef} {as : ActionScope} {leaf : Expr}
         | rGreater => simp [Cst.VariableDef.toActionScope?, Cst.VariableDef.toActionScopeAux?] at has
         | rGreaterEq => simp [Cst.VariableDef.toActionScope?, Cst.VariableDef.toActionScopeAux?] at has
         | rNotEq => simp [Cst.VariableDef.toActionScope?, Cst.VariableDef.toActionScopeAux?] at has
+        | rInvalidSingleEq => simp [Cst.VariableDef.toActionScope?, Cst.VariableDef.toActionScopeAux?] at has
   all_goals simp [Cst.VariableDef.toActionScope?, Cst.VariableDef.toActionScopeAux?] at has
 
 /-- Successful policy translation makes the translated CST expression and the AST
